src/Std/Data/DTreeMap/Internal/WF/Defs.lean
@@ -80,23 +80,23 @@ theorem WF.eraseManyEntries [Ord α] {ρ} [ForIn Id ρ ((a : α) × β a)] {t : 
     WF (t.eraseManyEntries l h).val :=
   (t.eraseManyEntries l h).2 hwf fun _ _ _ hwf' => hwf'.erase
 
-theorem WF.eraseMany [Ord α] {ρ} [ForIn Id ρ α] {t : Impl α β} {l : ρ} {h} (hwf : WF t) :
+theorem WF.eraseMany [Ord α] {ρ} [ForIn Id ρ α] [ForInNew Id ρ α] {t : Impl α β} {l : ρ} {h} (hwf : WF t) :
     WF (t.eraseMany l h).val :=
   (t.eraseMany l h).2 hwf fun _ _ _ hwf' => hwf'.erase
 
-theorem WF.insertMany [Ord α] {ρ} [ForIn Id ρ ((a : α) × β a)] {t : Impl α β} {l : ρ} {h} (hwf : WF t) :
+theorem WF.insertMany [Ord α] {ρ} [ForIn Id ρ ((a : α) × β a)] [ForInNew Id ρ ((a : α) × β a)] {t : Impl α β} {l : ρ} {h} (hwf : WF t) :
     WF (t.insertMany l h).val :=
   (t.insertMany l h).2 hwf fun _ _ _ _ hwf' => hwf'.insert
 
-theorem WF.insertManyIfNew [Ord α] {ρ} [ForIn Id ρ ((a : α) × β a)] {t : Impl α β} {l : ρ} {h} (hwf : WF t) :
+theorem WF.insertManyIfNew [Ord α] {ρ} [ForIn Id ρ ((a : α) × β a)] [ForInNew Id ρ ((a : α) × β a)] {t : Impl α β} {l : ρ} {h} (hwf : WF t) :
     WF (t.insertManyIfNew l h).val :=
   (t.insertManyIfNew l h).2 hwf fun _ _ _ _ hwf' => hwf'.insertIfNew
 
-theorem WF.constInsertMany [Ord α] {β : Type v} {ρ} [ForIn Id ρ (α × β)] {t : Impl α (fun _ => β)}
+theorem WF.constInsertMany [Ord α] {β : Type v} {ρ} [ForIn Id ρ (α × β)] [ForInNew Id ρ (α × β)] {t : Impl α (fun _ => β)}
     {l : ρ} {h} (hwf : WF t) : WF (Impl.Const.insertMany t l h).val :=
   (Impl.Const.insertMany t l h).2 hwf fun _ _ _ _ hwf' => hwf'.insert
 
-theorem WF.constInsertManyIfNewUnit [Ord α] {ρ} [ForIn Id ρ α] {t : Impl α (fun _ => Unit)} {l : ρ}
+theorem WF.constInsertManyIfNewUnit [Ord α] {ρ} [ForIn Id ρ α] [ForInNew Id ρ α] {t : Impl α (fun _ => Unit)} {l : ρ}
     {h} (hwf : WF t) : WF (Impl.Const.insertManyIfNewUnit t l h).val :=
   (Impl.Const.insertManyIfNewUnit t l h).2 hwf fun _ _ _ hwf' => hwf'.insertIfNew
 
